theories/lang/lang_extra.v
@@ -98,10 +98,8 @@ Section lang_extra.
 
 (** lemmas about transactions *)
 
-  Definition serialized_memory_descirptor l (r:VMID) ps := [l; (of_imm (encode_vmid r))]++ (map (λ pid, (of_pid pid)) ps).
-
   Definition serialized_transaction_descriptor (v r:VMID) (wf  l : Word) (ps: list PID) (h : Word): list Word :=
-    [(of_imm (encode_vmid v)); wf; h] ++ (serialized_memory_descirptor l r ps).
+    [(of_imm (encode_vmid v)); wf; h;l; (of_imm (encode_vmid r))] ++ (map (λ pid, (of_pid pid)) ps).
 
   Lemma trans_desc_length{i j wf l ps wh} des :
     des = serialized_transaction_descriptor i j wf  l ps wh ->
@@ -109,12 +107,13 @@ Section lang_extra.
     ((Z.of_nat (length des)) = 5 + (finz.to_z l))%Z.
   Proof.
     intros.
-    rewrite H /serialized_transaction_descriptor /serialized_memory_descirptor H0.
+    rewrite H /serialized_transaction_descriptor H0.
     simpl.
     rewrite fmap_length.
     lia.
   Qed.
 
+  (* TODO: reclaim this *)
   Lemma mem_desc_valid{ b psd σ} l (ps : list PID):
    l = (length ps) ->
    psd = (map (λ pid, (of_pid pid)) ps) ->
@@ -179,108 +178,111 @@ Section lang_extra.
     rewrite IHl //.
   Qed.
 
+  (* TODO: reprove this *)
   Lemma transaction_descriptor_valid{i j wf l psd σ} des p :
     (finz.to_z l) = (Z.of_nat (length psd)) ->
     des = serialized_transaction_descriptor i j wf l psd W0 ->
     seq_in_page (of_pid p) (length des) p ->
     (∀ (k : nat) (y1 y2 : Addr),
        finz.seq (of_pid p) (length des) !! k = Some y1 → des !! k = Some y2 → get_mem σ !! y1 = Some y2) ->
-    parse_transaction_descriptor σ p = Some (i , None, wf,  j , list_to_set psd).
+    parse_transaction_descriptor σ p (length des) = Some (i, None, wf, j, list_to_set psd).
   Proof.
-    intros.
-    rewrite /parse_transaction_descriptor /get_memory_with_offset.
-    destruct H1 as [_ [_ [? _]]].
-    pose proof (trans_desc_length des H0 H) as Hlen.
-    assert (HpSome: ((of_pid p) + 0)%f = Some ((of_pid p) ^+ 0)%f).
-    solve_finz.
-    rewrite HpSome //=;clear HpSome.
-    rewrite (H2 0 ((of_pid p) ^+ 0)%f (encode_vmid i)).
-    2: { apply finz_seq_lookup. lia. solve_finz. }
-    2: { rewrite H0 /serialized_transaction_descriptor. by list_simplifier. }
-    assert (HpSome: ((of_pid p) + 1)%f = Some ((of_pid p) ^+ 1)%f).
-    solve_finz.
-    rewrite HpSome //=;clear HpSome.
-    rewrite (H2 1 ((of_pid p) ^+ 1)%f wf).
-    2: { apply finz_seq_lookup. lia. solve_finz. }
-    2: { rewrite H0 /serialized_transaction_descriptor. by list_simplifier. }
-    assert (HpSome: ((of_pid p) + 2)%f = Some ((of_pid p) ^+ 2)%f).
-    solve_finz.
-    rewrite HpSome //=;clear HpSome.
-    rewrite (H2 2 ((of_pid p) ^+ 2)%f W0).
-    2: { apply finz_seq_lookup. lia. solve_finz. }
-    2: { rewrite H0 /serialized_transaction_descriptor. by list_simplifier. }
-    rewrite  /parse_memory_region_descriptor /get_memory_with_offset.
-    assert (HpSome: ((of_pid p) ^+ 3 + 0)%f = Some ((of_pid p) ^+ 3)%f).
-    solve_finz.
-    rewrite HpSome //=;clear HpSome.
-    rewrite (H2 3 ((of_pid p) ^+ 3)%f l).
-    2: { apply finz_seq_lookup. lia. solve_finz. }
-    2: { rewrite H0 /serialized_transaction_descriptor. by list_simplifier. }
-    assert (HpSome: ((of_pid p) ^+ 3 + 1)%f = Some ((of_pid p) ^+ 4)%f).
-    solve_finz.
-    rewrite HpSome //=;clear HpSome.
-    rewrite (H2 4 ((of_pid p) ^+ 4)%f (encode_vmid j)).
-    2: { apply finz_seq_lookup. lia. solve_finz. }
-    2: { rewrite H0 /serialized_transaction_descriptor. by list_simplifier. }
-    rewrite !decode_encode_vmid /parse_list_of_pids /= .
-    rewrite (@mem_desc_valid _ (map (λ pid, (of_pid pid)) psd) _ _ psd );eauto.
-    2: { lia. }
-    2: { intros.
-         apply (H2 (k+5) _).
-         assert (Hlenmapeq: length ( map (λ pid : PID, (of_pid pid)) psd) = length psd).
-        apply fmap_length.
-         apply (finz_seq_lookup _ y1).
-         assert (Hklt: k < length ( map (λ pid : PID, (of_pid pid)) psd)).
-         rewrite <-(finz_seq_length ((p ^+ 3) ^+ 2)%f).
-         apply lookup_lt_is_Some.
-         by exists y1.
-        rewrite Hlenmapeq in Hklt.
-        lia.
-        apply (finz_seq_lookup' _ y1 k _ ) in H3.
-        2: { rewrite Hlenmapeq. solve_finz. }
-        destruct H3.
-        solve_finz.
-        rewrite H0 /serialized_transaction_descriptor.
-        simpl.
-        rewrite !lookup_cons_ne_0; try lia.
-        rewrite -H4.
-        f_equal.
-        lia.
-       }
-    rewrite -> sequence_a_map_unit.
-    done.
-  Qed.
+    Admitted.
+  (*   intros. *)
+  (*   rewrite /parse_transaction_descriptor /get_memory_with_offset. *)
+  (*   destruct H1 as [_ [_ [? _]]]. *)
+  (*   pose proof (trans_desc_length des H0 H) as Hlen. *)
+  (*   assert (HpSome: ((of_pid p) + 0)%f = Some ((of_pid p) ^+ 0)%f). *)
+  (*   solve_finz. *)
+  (*   rewrite HpSome //=;clear HpSome. *)
+  (*   rewrite (H2 0 ((of_pid p) ^+ 0)%f (encode_vmid i)). *)
+  (*   2: { apply finz_seq_lookup. lia. solve_finz. } *)
+  (*   2: { rewrite H0 /serialized_transaction_descriptor. by list_simplifier. } *)
+  (*   assert (HpSome: ((of_pid p) + 1)%f = Some ((of_pid p) ^+ 1)%f). *)
+  (*   solve_finz. *)
+  (*   rewrite HpSome //=;clear HpSome. *)
+  (*   rewrite (H2 1 ((of_pid p) ^+ 1)%f wf). *)
+  (*   2: { apply finz_seq_lookup. lia. solve_finz. } *)
+  (*   2: { rewrite H0 /serialized_transaction_descriptor. by list_simplifier. } *)
+  (*   assert (HpSome: ((of_pid p) + 2)%f = Some ((of_pid p) ^+ 2)%f). *)
+  (*   solve_finz. *)
+  (*   rewrite HpSome //=;clear HpSome. *)
+  (*   rewrite (H2 2 ((of_pid p) ^+ 2)%f W0). *)
+  (*   2: { apply finz_seq_lookup. lia. solve_finz. } *)
+  (*   2: { rewrite H0 /serialized_transaction_descriptor. by list_simplifier. } *)
+  (*   rewrite  /parse_memory_region_descriptor /get_memory_with_offset. *)
+  (*   assert (HpSome: ((of_pid p) ^+ 3 + 0)%f = Some ((of_pid p) ^+ 3)%f). *)
+  (*   solve_finz. *)
+  (*   rewrite HpSome //=;clear HpSome. *)
+  (*   rewrite (H2 3 ((of_pid p) ^+ 3)%f l). *)
+  (*   2: { apply finz_seq_lookup. lia. solve_finz. } *)
+  (*   2: { rewrite H0 /serialized_transaction_descriptor. by list_simplifier. } *)
+  (*   assert (HpSome: ((of_pid p) ^+ 3 + 1)%f = Some ((of_pid p) ^+ 4)%f). *)
+  (*   solve_finz. *)
+  (*   rewrite HpSome //=;clear HpSome. *)
+  (*   rewrite (H2 4 ((of_pid p) ^+ 4)%f (encode_vmid j)). *)
+  (*   2: { apply finz_seq_lookup. lia. solve_finz. } *)
+  (*   2: { rewrite H0 /serialized_transaction_descriptor. by list_simplifier. } *)
+  (*   rewrite !decode_encode_vmid /parse_list_of_pids /= . *)
+  (*   rewrite (@mem_desc_valid _ (map (λ pid, (of_pid pid)) psd) _ _ psd );eauto. *)
+  (*   2: { lia. } *)
+  (*   2: { intros. *)
+  (*        apply (H2 (k+5) _). *)
+  (*        assert (Hlenmapeq: length ( map (λ pid : PID, (of_pid pid)) psd) = length psd). *)
+  (*       apply fmap_length. *)
+  (*        apply (finz_seq_lookup _ y1). *)
+  (*        assert (Hklt: k < length ( map (λ pid : PID, (of_pid pid)) psd)). *)
+  (*        rewrite <-(finz_seq_length ((p ^+ 3) ^+ 2)%f). *)
+  (*        apply lookup_lt_is_Some. *)
+  (*        by exists y1. *)
+  (*       rewrite Hlenmapeq in Hklt. *)
+  (*       lia. *)
+  (*       apply (finz_seq_lookup' _ y1 k _ ) in H3. *)
+  (*       2: { rewrite Hlenmapeq. solve_finz. } *)
+  (*       destruct H3. *)
+  (*       solve_finz. *)
+  (*       rewrite H0 /serialized_transaction_descriptor. *)
+  (*       simpl. *)
+  (*       rewrite !lookup_cons_ne_0; try lia. *)
+  (*       rewrite -H4. *)
+  (*       f_equal. *)
+  (*       lia. *)
+  (*      } *)
+  (*   rewrite -> sequence_a_map_unit. *)
+  (*   done. *)
+  (* Qed. *)
 
   Lemma transaction_retrieve_descriptor_valid {j handle wf σ} des p :
-    des = [of_imm (encode_vmid j); wf; handle; of_imm (encode_vmid (get_current_vm σ))]->
+    des = [of_imm (encode_vmid j); wf; handle; of_imm (encode_vmid (get_current_vm σ))] ->
     seq_in_page (of_pid p) (length des) p ->
     (∀ (k : nat) (y1 y2 : Addr),
              finz.seq (of_pid p) (length des) !! k = Some y1 → des !! k = Some y2 → get_mem σ !! y1 = Some y2) ->
-    parse_transaction_descriptor_retrieve σ p = Some (j, Some handle, wf, (get_current_vm σ), ∅).
+    parse_transaction_descriptor_retrieve σ p (length des)  = Some (j, Some handle, wf, (get_current_vm σ), ∅).
   Proof.
-    intros H H0 H1.
-    rewrite /parse_transaction_descriptor_retrieve /get_memory_with_offset.
-    destruct H0 as [_ [? _]].
-    simpl.
-    pose proof (last_addr_in_bound p) as HSome.
-    assert ( ((of_pid p) + 0)%f = Some ((of_pid p) ^+ 0)%f) as ->.
-    solve_finz.
-    rewrite (H1 0 ((of_pid p) ^+ 0)%f (encode_vmid j)).
-    2: { apply finz_seq_lookup. rewrite H /=. lia. solve_finz. }
-    2: { rewrite H. by list_simplifier. }
-    assert (((of_pid p) + 1)%f = Some ((of_pid p) ^+ 1)%f) as ->.
-    solve_finz.
-    rewrite (H1 1 ((of_pid p) ^+ 1)%f wf).
-    2: { apply finz_seq_lookup. rewrite H /=. lia. solve_finz. }
-    2: { rewrite H . by list_simplifier. }
-    assert (((of_pid p) + 2)%f = Some ((of_pid p) ^+ 2)%f) as ->.
-    solve_finz.
-    rewrite (H1 2 ((of_pid p) ^+ 2)%f handle).
-    2: { apply finz_seq_lookup. rewrite H /=. lia. solve_finz. }
-    2: { rewrite H. by list_simplifier. }
-    rewrite !decode_encode_vmid /=.
-    reflexivity.
-  Qed.
+    Admitted.
+  (*   intros H H0 H1. *)
+  (*   rewrite /parse_transaction_descriptor_retrieve /get_memory_with_offset. *)
+  (*   destruct H0 as [_ [? _]]. *)
+  (*   simpl. *)
+  (*   pose proof (last_addr_in_bound p) as HSome. *)
+  (*   assert ( ((of_pid p) + 0)%f = Some ((of_pid p) ^+ 0)%f) as ->. *)
+  (*   solve_finz. *)
+  (*   rewrite (H1 0 ((of_pid p) ^+ 0)%f (encode_vmid j)). *)
+  (*   2: { apply finz_seq_lookup. rewrite H /=. lia. solve_finz. } *)
+  (*   2: { rewrite H. by list_simplifier. } *)
+  (*   assert (((of_pid p) + 1)%f = Some ((of_pid p) ^+ 1)%f) as ->. *)
+  (*   solve_finz. *)
+  (*   rewrite (H1 1 ((of_pid p) ^+ 1)%f wf). *)
+  (*   2: { apply finz_seq_lookup. rewrite H /=. lia. solve_finz. } *)
+  (*   2: { rewrite H . by list_simplifier. } *)
+  (*   assert (((of_pid p) + 2)%f = Some ((of_pid p) ^+ 2)%f) as ->. *)
+  (*   solve_finz. *)
+  (*   rewrite (H1 2 ((of_pid p) ^+ 2)%f handle). *)
+  (*   2: { apply finz_seq_lookup. rewrite H /=. lia. solve_finz. } *)
+  (*   2: { rewrite H. by list_simplifier. } *)
+  (*   rewrite !decode_encode_vmid /=. *)
+  (*   reflexivity. *)
+  (* Qed. *)
 
 
   (** lemmas about taking a step *)
